Removing admits

theories/Interaction_Between_Lts/Examples_of_Interactions/ParallelLTSConstruction.v
@@ -23,7 +23,7 @@
    SOFTWARE.
 *)
 
-From Coq.Unicode Require Import Utf8.
+From Stdlib.Unicode Require Import Utf8.
 From stdpp Require Import base.
 From Must Require Import gLts InteractionBetweenLts.
 
@@ -31,3 +31,41 @@ From Must Require Import gLts InteractionBetweenLts.
 
 #[global] Program Instance parallel_gLts {P1 P2}
  `{Prop_of_Inter P1 P2 A dual} : gLts (P1 * P2) H := inter_lts dual.
+
+Definition reverse_dual `{H : !ExtAction A} μ1 μ2 := dual μ2 μ1.
+
+#[global] Program Instance Inter_rev_parallel `{Prop_of_Inter P1 P2 A dual} : Prop_of_Inter P2 P1 A reverse_dual.
+Next Obligation.
+  intros. destruct H2. exact (lts_essential_actions_right X).
+Defined.
+Next Obligation.
+  intros. simpl in *. unfold Inter_rev_parallel_obligation_1 in H3.
+  destruct H2. simpl in *. eauto.
+Defined.
+Next Obligation.
+  intros. destruct H2. exact (lts_essential_actions_left X).
+Defined.
+Next Obligation.
+  intros. destruct H2; eauto.
+Defined.
+Next Obligation.
+  intros. unfold Inter_rev_parallel_obligation_1.
+  unfold Inter_rev_parallel_obligation_3. destruct H2; eauto.
+  unfold reverse_dual in H5. eapply lts_essential_actions_spec_interact in H5; eauto.
+  destruct H5. right; eauto. left; eauto.
+Defined.
+Next Obligation.
+  intros. destruct H2. exact (lts_co_inter_action_right X X0).
+Defined.
+Next Obligation.
+  intros. unfold Inter_rev_parallel_obligation_6. destruct H2; eauto.
+Defined.
+Next Obligation.
+  intros. destruct H2. exact (lts_co_inter_action_left X X0).
+Defined.
+Next Obligation.
+  intros. unfold Inter_rev_parallel_obligation_8. destruct H2; eauto.
+Defined.
+
+ #[global] Program Instance parallel_gLts_inv {P1 P2}
+ `{Prop_of_Inter P1 P2 A dual} : gLts (P2 * P1) H := inter_lts reverse_dual.
