theories/Generalization/Old_Developments/OldTransitionSystems.v
@@ -23,7 +23,7 @@
 *)
 
 
-From Coq.Unicode Require Import Utf8. 
+From Stdlib.Unicode Require Import Utf8. 
 From stdpp Require Import countable gmap finite decidable gmultiset.
 From Must Require Import InputOutputActions ActTau.
 
