theories/Labelled_Transition_System/Examples_of_LTS/VACCS/VACCS_Instance.v
@@ -5132,3 +5132,5 @@ Next Obligation.
     destruct H. rewrite VarC_add_zero_ext in H. exists x. destruct H. split ;eauto.
 Qed.
 
+
+
