theories/Testing_Pre_orders/Must/Alternative_Preorder/Acceptance_Set/DefinitionAS.v
@@ -23,8 +23,8 @@
    SOFTWARE.
 *)
 
-From Coq.Unicode Require Import Utf8.
-From Coq.Program Require Import Equality.
+From Stdlib.Unicode Require Import Utf8.
+From Stdlib.Program Require Import Equality.
 From stdpp Require Import finite gmap decidable.
 From Must Require Import ActTau gLts Bisimulation Lts_OBA Subset_Act WeakTransitions Testing_Predicate
     StateTransitionSystems InteractionBetweenLts Convergence Termination FiniteImageLTS.
